denote Grammar commutes with derive in OriginalTotal

Validator/Derive/Enter.lean
@@ -1,21 +1,22 @@
-import Validator.Expr.Expr
+import Validator.Expr.Regex
+import Validator.Expr.Grammar
 import Validator.Expr.IfExpr
 
 namespace Enter
 
-def enter (x: Expr μ α) (res: IfExprs μ α := []): IfExprs μ α :=
+def enter (x: Rule μ α Pred) (res: IfExprs μ α := []): IfExprs μ α :=
   match x with
-  | Expr.emptyset => res
-  | Expr.epsilon => res
-  | Expr.tree pred childRef => (IfExpr.mk pred childRef) :: res
-  | Expr.or y z => enter y (enter z res)
-  | Expr.concat y z =>
-    if Expr.nullable y
+  | Regex.emptyset => res
+  | Regex.emptystr => res
+  | Regex.symbol (pred, childRef) => (IfExpr.mk pred childRef) :: res
+  | Regex.or y z => enter y (enter z res)
+  | Regex.concat y z =>
+    if Regex.nullable y
     then enter y (enter z res)
     else enter y res
-  | Expr.star y => enter y res
+  | Regex.star y => enter y res
 
-def deriveEnter (xs: Exprs μ α): IfExprs μ α :=
+def deriveEnter (xs: Rules μ α Pred): IfExprs μ α :=
   List.flatten (List.map Enter.enter xs)
 
 theorem deriveEnter_nil_is_nil {α: Type} {μ: Nat}:
@@ -23,10 +24,10 @@ theorem deriveEnter_nil_is_nil {α: Type} {μ: Nat}:
   unfold deriveEnter
   simp
 
-theorem deriveEnter_cons_is_concat {α: Type} (x: Expr μ α) (xs: Exprs μ α):
+theorem deriveEnter_cons_is_concat {α: Type} (x: Rule μ α Pred) (xs: Rules μ α Pred):
   deriveEnter (x::xs) = (deriveEnter [x]) ++ (deriveEnter xs) := by
   unfold deriveEnter
   simp
 
 class DeriveEnter (m: Type -> Type u) (μ: Nat) (α: outParam Type)  where
-  deriveEnter (xs: Exprs μ α): m (IfExprs μ α)
+  deriveEnter (xs: Rules μ α Pred): m (IfExprs μ α)
