Validator/Expr/Grammar.lean
@@ -16,6 +16,9 @@ abbrev Ref μ := Fin μ -- non-terminal
 abbrev Rule (μ: Nat) (α: Type) (Φ: (α: Type) -> Type) :=
   Regex (Φ α × Ref μ)
 
+abbrev Rules (μ: Nat) (α: Type) (Φ: (α: Type) -> Type) :=
+  List (Rule μ α Φ)
+
 structure Grammar (μ: Nat) (α: Type) (Φ: (α: Type) -> Type) where
   start: Rule μ α Φ
   prods: Vector (Rule μ α Φ) μ
@@ -63,7 +66,7 @@ def example_grammar: Grammar 1 Char Pred :=
   example_grammar.lookup (Fin.mk 0 (by omega))
   = Regex.emptystr
 
-theorem denote_rule_decreasing {x: Hedge.Node α} {xs: Hedge α} (h: List.IsInfix [x] xs):
+theorem Rule.denote_decreasing {x: Hedge.Node α} {xs: Hedge α} (h: List.IsInfix [x] xs):
   sizeOf x.getChildren < sizeOf xs := by
   cases x with
   | mk label children =>
@@ -73,30 +76,30 @@ theorem denote_rule_decreasing {x: Hedge.Node α} {xs: Hedge α} (h: List.IsInfi
   simp +arith only at h
   omega
 
-def denote_rule {α: Type} [BEq α] (g: Grammar μ α Pred) (r: Rule μ α Pred) (xs: Hedge α): Prop :=
+def Rule.denote {α: Type} [BEq α] (g: Grammar μ α Pred) (r: Rule μ α Pred) (xs: Hedge α): Prop :=
   Regex.denote_infix r xs (fun (pred, ref) xs' =>
     match xs' with
     | Subtype.mk [x] _hx =>
         Pred.eval pred x.getLabel
-        /\ denote_rule g (g.lookup ref) x.getChildren
+        /\ Rule.denote g (g.lookup ref) x.getChildren
     | _ => False
   )
   termination_by xs
-  decreasing_by exact (denote_rule_decreasing _hx)
+  decreasing_by exact (Rule.denote_decreasing _hx)
 
 def Grammar.denote {α: Type} [BEq α] (g: Grammar μ α Pred) (xs: Hedge α): Prop :=
-  denote_rule g g.start xs
+  Rule.denote g g.start xs
 
 theorem simp_denote_rule' {α: Type} [BEq α] (g: Grammar μ α Pred) (r: Rule μ α Pred) (xs: Hedge α):
   (Regex.denote_infix r xs (fun (pred, ref) xs' =>
     match xs' with
     | Subtype.mk [x] _hx =>
         Pred.eval pred x.getLabel
-        /\ denote_rule g (g.lookup ref) x.getChildren
+        /\ Rule.denote g (g.lookup ref) x.getChildren
     | _ => False
   )) =
   (Regex.denote_infix r xs (fun (pred, ref) xs' =>
-    ∃ x: Hedge.Node α, xs'.val = [x] /\ Pred.eval pred x.getLabel /\ denote_rule g (g.lookup ref) x.getChildren
+    ∃ x: Hedge.Node α, xs'.val = [x] /\ Pred.eval pred x.getLabel /\ Rule.denote g (g.lookup ref) x.getChildren
   )) := by
   congr
   ext s xs'
@@ -116,11 +119,11 @@ theorem simp_denote_rule' {α: Type} [BEq α] (g: Grammar μ α Pred) (r: Rule �
       simp
 
 theorem simp_denote_rule {α: Type} [BEq α] (g: Grammar μ α Pred) (r: Rule μ α Pred) (xs: Hedge α):
-  denote_rule g r xs =
+  Rule.denote g r xs =
   Regex.denote_infix r xs (fun (pred, ref) xs' =>
-    ∃ label children, xs'.val = [Hedge.Node.mk label children] /\ Pred.eval pred label /\ denote_rule g (g.lookup ref) children
+    ∃ label children, xs'.val = [Hedge.Node.mk label children] /\ Pred.eval pred label /\ Rule.denote g (g.lookup ref) children
   ) := by
-  nth_rewrite 1 [denote_rule]
+  nth_rewrite 1 [Rule.denote]
   rw [simp_denote_rule']
   congr
   ext s xs'
@@ -138,39 +141,39 @@ theorem simp_denote_rule {α: Type} [BEq α] (g: Grammar μ α Pred) (r: Rule μ
     obtain ⟨label, children, hxs, h⟩ := h
     exists Hedge.Node.mk label children
 
-theorem Grammar.denote_rule_emptyset {α: Type} [BEq α] {g: Grammar μ α Pred}:
-  denote_rule g Regex.emptyset = Language.emptyset := by
+theorem Rule.denote_emptyset {α: Type} [BEq α] {g: Grammar μ α Pred}:
+  Rule.denote g Regex.emptyset = Language.emptyset := by
   unfold Language.emptyset
   funext xs
-  unfold denote_rule
+  unfold Rule.denote
   simp [Regex.denote_infix_emptyset]
 
-theorem Grammar.denote_rule_emptystr {α: Type} [BEq α] {g: Grammar μ α Pred}:
-  denote_rule g Regex.emptystr = Language.emptystr := by
+theorem Rule.denote_emptystr {α: Type} [BEq α] {g: Grammar μ α Pred}:
+  Rule.denote g Regex.emptystr = Language.emptystr := by
   unfold Language.emptystr
   funext xs
-  unfold denote_rule
+  unfold Rule.denote
   simp [Regex.denote_infix_emptystr]
 
 theorem denote_rule_symbol' {μ: Nat} {α: Type} [BEq α]
   {g: Grammar μ α Pred} {pred: Pred α} {ref: Ref μ} {xs: Hedge α}:
-  denote_rule g (Regex.symbol (pred, ref)) xs
-  <-> Language.tree (Pred.eval pred) (denote_rule g (g.lookup ref)) xs := by
+  Rule.denote g (Regex.symbol (pred, ref)) xs
+  <-> Language.tree (Pred.eval pred) (Rule.denote g (g.lookup ref)) xs := by
   cases xs with
   | nil =>
     unfold Language.tree
-    unfold denote_rule
+    unfold Rule.denote
     simp [Regex.denote_infix_symbol]
   | cons x xs =>
     cases xs with
     | cons x' xs' =>
       unfold Language.tree
-      unfold denote_rule
+      unfold Rule.denote
       simp [Regex.denote_infix_symbol]
       simp [List.InfixOf.self]
     | nil =>
       unfold Language.tree
-      unfold denote_rule
+      unfold Rule.denote
       simp [Regex.denote_infix_symbol]
       simp [List.InfixOf.self]
       apply Iff.intro
@@ -184,7 +187,7 @@ theorem denote_rule_symbol' {μ: Nat} {α: Type} [BEq α]
         simp [Hedge.Node.getLabel] at hp
         simp [Hedge.Node.getChildren] at hg
         apply And.intro hp
-        rw [<- denote_rule]
+        rw [<- Rule.denote]
         exact hg
       case mpr h =>
         intro h
@@ -196,32 +199,32 @@ theorem denote_rule_symbol' {μ: Nat} {α: Type} [BEq α]
         rw [hl, hc] at *
         clear hl hc label' children'
         simp [Hedge.Node.getChildren, Hedge.Node.getLabel]
-        rw [<- denote_rule] at hg
+        rw [<- Rule.denote] at hg
         apply And.intro hp hg
 
-theorem Grammar.denote_rule_symbol {μ: Nat} {α: Type} [BEq α]
+theorem Rule.denote_symbol {μ: Nat} {α: Type} [BEq α]
   {g: Grammar μ α Pred} {pred: Pred α} {ref: Ref μ}:
-  denote_rule g (Regex.symbol (pred, ref))
-  = Language.tree (Pred.eval pred) (denote_rule g (g.lookup ref)) := by
+  Rule.denote g (Regex.symbol (pred, ref))
+  = Language.tree (Pred.eval pred) (Rule.denote g (g.lookup ref)) := by
   funext xs
   rw [denote_rule_symbol']
 
-theorem Grammar.denote_rule_or {μ: Nat} {α: Type} [BEq α]
+theorem Rule.denote_or {μ: Nat} {α: Type} [BEq α]
   {g: Grammar μ α Pred} {p q: Rule μ α Pred}:
-  denote_rule g (Regex.or p q)
-  = Language.or (denote_rule g p) (denote_rule g q) := by
+  Rule.denote g (Regex.or p q)
+  = Language.or (Rule.denote g p) (Rule.denote g q) := by
   funext xs
   unfold Language.or
-  unfold denote_rule
+  unfold Rule.denote
   simp [Regex.denote_infix_or]
 
-theorem Grammar.denote_rule_concat_n {μ: Nat} {α: Type} [BEq α]
+theorem Rule.denote_concat_n {μ: Nat} {α: Type} [BEq α]
   {g: Grammar μ α Pred} {p q: Rule μ α Pred}:
-  denote_rule g (Regex.concat p q)
-  = Language.concat_n (denote_rule g p) (denote_rule g q) := by
+  Rule.denote g (Regex.concat p q)
+  = Language.concat_n (Rule.denote g p) (Rule.denote g q) := by
   funext xs
   unfold Language.concat_n
-  unfold denote_rule
+  unfold Rule.denote
   simp only [Regex.denote_infix_concat_n]
   congr
   ext n
@@ -260,14 +263,22 @@ theorem Grammar.denote_rule_concat_n {μ: Nat} {α: Type} [BEq α]
       | cons _ _ =>
         simp
 
+theorem Rule.denote_concat {μ: Nat} {α: Type} [BEq α]
+  {g: Grammar μ α Pred} {p q: Rule μ α Pred}:
+  Rule.denote g (Regex.concat p q)
+  = Language.concat (Rule.denote g p) (Rule.denote g q) := by
+  rw [Rule.denote_concat_n]
+  funext xs
+  rw [Language.concat_is_concat_n]
+
 theorem denote_rule_star_n' {μ: Nat} {α: Type} [BEq α]
   {g: Grammar μ α Pred} {r: Rule μ α Pred} (xs: Hedge α):
-  denote_rule g (Regex.star r) xs
+  Rule.denote g (Regex.star r) xs
   <->
-  Language.star_n (denote_rule g r) xs := by
+  Language.star_n (Rule.denote g r) xs := by
   rw [<- eq_iff_iff]
   unfold Language.star_n
-  unfold denote_rule
+  unfold Rule.denote
   cases xs with
   | nil =>
     simp [Regex.denote_infix_star_n]
@@ -302,7 +313,7 @@ theorem denote_rule_star_n' {μ: Nat} {α: Type} [BEq α]
       unfold List.InfixOf.mk
       simp
       rw [<- denote_rule_star_n']
-      rw [denote_rule]
+      rw [Rule.denote]
       rw [<- eq_iff_iff]
       congr
       ext s ys
@@ -322,13 +333,39 @@ theorem denote_rule_star_n' {μ: Nat} {α: Type} [BEq α]
     obtain ⟨n, hn⟩ := n
     apply List.list_length_drop_lt_cons
 
-theorem Grammar.denote_rule_star_n {μ: Nat} {α: Type} [BEq α]
+theorem Rule.denote_star_n {μ: Nat} {α: Type} [BEq α]
   {g: Grammar μ α Pred} {r: Rule μ α Pred}:
-  denote_rule g (Regex.star r)
+  Rule.denote g (Regex.star r)
   =
-  Language.star_n (denote_rule g r) := by
+  Language.star_n (Rule.denote g r) := by
   funext xs
   rw [denote_rule_star_n']
+
+theorem Rule.denote_star {μ: Nat} {α: Type} [BEq α]
+  {g: Grammar μ α Pred} {r: Rule μ α Pred}:
+  Rule.denote g (Regex.star r)
+  =
+  Language.star (Rule.denote g r) := by
+  funext xs
+  rw [denote_rule_star_n']
+  rw [Language.star_is_star_n]
+
+def Rule.denote_onlyif {α: Type} [BEq α] (condition: Prop) [dcond: Decidable condition] (g: Grammar μ α Pred) (x: Rule μ α Pred):
+  denote g (Regex.onlyif condition x) = Language.onlyif condition (denote g x) := by
+  unfold Language.onlyif
+  unfold Regex.onlyif
+  funext xs
+  split_ifs
+  case pos hc =>
+    simp only [eq_iff_iff, iff_and_self]
+    intro d
+    assumption
+  case neg hc =>
+    simp only [eq_iff_iff]
+    rw [Rule.denote, Regex.denote_infix]
+    simp only [Language.emptyset, false_iff, not_and]
+    intro hc'
+    contradiction
 
 def Rule.nullable (r: Rule μ α Φ): Bool :=
   Regex.nullable r
@@ -336,90 +373,51 @@ def Rule.nullable (r: Rule μ α Φ): Bool :=
 def Grammar.nullable (g: Grammar μ α Φ): Bool :=
   Rule.nullable g.start
 
-theorem decreasing_or_l {α: Type} {σ: Type} [SizeOf σ] (r1 r2: Regex σ) (x: Hedge.Node α):
-  Prod.Lex
-    (fun a₁ a₂ => sizeOf a₁ < sizeOf a₂)
-    (fun a₁ a₂ => sizeOf a₁ < sizeOf a₂)
-    (x, r1)
-    (x, Regex.or r1 r2) := by
-  apply Prod.Lex.right
-  simp +arith only [Regex.or.sizeOf_spec]
-
-theorem decreasing_or_r {α: Type} {σ: Type} [SizeOf σ] (r1 r2: Regex σ) (x: Hedge.Node α):
-  Prod.Lex
-    (fun a₁ a₂ => sizeOf a₁ < sizeOf a₂)
-    (fun a₁ a₂ => sizeOf a₁ < sizeOf a₂)
-    (x, r2)
-    (x, Regex.or r1 r2) := by
-  apply Prod.Lex.right
-  simp +arith only [Regex.or.sizeOf_spec]
-
-theorem decreasing_concat_l {α: Type} {σ: Type} [SizeOf σ] (r1 r2: Regex σ) (x: Hedge.Node α):
-  Prod.Lex
-    (fun a₁ a₂ => sizeOf a₁ < sizeOf a₂)
-    (fun a₁ a₂ => sizeOf a₁ < sizeOf a₂)
-    (x, r1)
-    (x, Regex.concat r1 r2) := by
-  apply Prod.Lex.right
-  simp +arith only [Regex.concat.sizeOf_spec]
-
-theorem decreasing_concat_r {α: Type} {σ: Type} [SizeOf σ] (r1 r2: Regex σ) (x: Hedge.Node α):
-  Prod.Lex
-    (fun a₁ a₂ => sizeOf a₁ < sizeOf a₂)
-    (fun a₁ a₂ => sizeOf a₁ < sizeOf a₂)
-    (x, r2)
-    (x, Regex.concat r1 r2) := by
-  apply Prod.Lex.right
-  simp +arith only [Regex.concat.sizeOf_spec]
-
-theorem decreasing_star {α: Type} {σ: Type} [SizeOf σ] (r: Regex σ) (x: Hedge.Node α):
-  Prod.Lex
-    (fun a₁ a₂ => sizeOf a₁ < sizeOf a₂)
-    (fun a₁ a₂ => sizeOf a₁ < sizeOf a₂)
-    (x, r)
-    (x, Regex.star r) := by
-  apply Prod.Lex.right
-  simp +arith only [Regex.star.sizeOf_spec]
-
-theorem decreasing_symbol {α: Type} {σ: Type} [SizeOf σ] (r1 r2: Regex σ) (label: α) (children: Hedge α) (x: Hedge.Node α) (h: x ∈ children):
-  Prod.Lex
-    (fun a₁ a₂ => sizeOf a₁ < sizeOf a₂)
-    (fun a₁ a₂ => sizeOf a₁ < sizeOf a₂)
-    (x, r1)
-    (Hedge.Node.mk label children, r2) := by
-  apply Prod.Lex.left
-  simp +arith only [Hedge.Node.mk.sizeOf_spec]
-  have h' := List.list_elem_lt h
-  omega
-
-def Rule.derive [BEq α] [DecidableEq α] (g: Grammar μ α Pred) (r: Rule μ α Pred) (x: Hedge.Node α): Rule μ α Pred :=
-  match r with
-  | Regex.emptyset => Regex.emptyset
-  | Regex.emptystr => Regex.emptyset
-  | Regex.symbol (p, ref) =>
-    match x with
-    | Hedge.Node.mk label children =>
-      Regex.onlyif
-        (
-          Pred.eval p label
-          /\ Rule.nullable (List.foldl (Rule.derive g) (g.lookup ref) children)
-        )
-        Regex.emptystr
-  | Regex.or r1 r2 =>
-    Regex.or (Rule.derive g r1 x) (Rule.derive g r2 x)
-  | Regex.concat r1 r2 =>
-    Regex.or
-      (Regex.concat (Rule.derive g r1 x) r2)
-      (Regex.onlyif (Rule.nullable r1) (Rule.derive g r2 x))
-  | Regex.star r1 =>
-    Regex.concat (Rule.derive g r1 x) (Regex.star r1)
-  termination_by (x, r)
-  decreasing_by
-    · apply decreasing_symbol (h := by assumption)
-    · apply decreasing_symbol (h := by assumption)
-    · apply decreasing_symbol (h := by assumption)
-    · apply decreasing_or_l
-    · apply decreasing_or_r
-    · apply decreasing_concat_l
-    · apply decreasing_concat_r
-    · apply decreasing_star
+theorem Rule.null_commutes {α: Type} [BEq α] (g: Grammar μ α Pred) (x: Rule μ α Pred):
+  ((Rule.nullable x) = true) = Language.null (denote g x) := by
+  induction x with
+  | emptyset =>
+    rw [denote_emptyset]
+    rw [Language.null_emptyset]
+    unfold Rule.nullable
+    unfold Regex.nullable
+    apply Bool.false_eq_true
+  | emptystr =>
+    rw [denote_emptystr]
+    rw [Language.null_emptystr]
+    unfold Rule.nullable
+    unfold Regex.nullable
+    simp only
+  | symbol s =>
+    obtain ⟨p, children⟩ := s
+    rw [denote_symbol]
+    rw [Language.null_tree]
+    unfold Rule.nullable
+    unfold Regex.nullable
+    apply Bool.false_eq_true
+  | or p q ihp ihq =>
+    rw [denote_or]
+    rw [Language.null_or]
+    unfold Rule.nullable
+    unfold Regex.nullable
+    rw [<- ihp]
+    rw [<- ihq]
+    unfold Rule.nullable
+    unfold Regex.nullable
+    rw [Bool.or_eq_true]
+  | concat p q ihp ihq =>
+    rw [denote_concat]
+    rw [Language.null_concat]
+    unfold Rule.nullable
+    unfold Regex.nullable
+    rw [<- ihp]
+    rw [<- ihq]
+    unfold Rule.nullable
+    unfold Regex.nullable
+    rw [Bool.and_eq_true]
+  | star r ih =>
+    rw [denote_star]
+    rw [Language.null_star]
+    unfold Rule.nullable
+    unfold Regex.nullable
+    simp only
