Validator/Expr/IfExpr.lean
@@ -1,5 +1,6 @@
 import Validator.Expr.Pred
-import Validator.Expr.Expr
+import Validator.Expr.Regex
+import Validator.Expr.Grammar
 
 inductive IfExpr μ α where
   | mk (cnd: Pred α) (thn: Fin μ)
@@ -8,22 +9,22 @@ abbrev IfExprs μ α := List (IfExpr μ α)
 
 namespace IfExpr
 
-def eval {α: Type} [DecidableEq α] (g: Expr.Grammar μ α) (ifExpr: IfExpr μ α) (t: α): Expr μ α :=
+def eval {α: Type} [DecidableEq α] (g: Grammar μ α Pred) (ifExpr: IfExpr μ α) (t: α): Rule μ α Pred :=
   match ifExpr with
   | IfExpr.mk cnd thn =>
     if Pred.eval cnd t
     then g.lookup thn
-    else Expr.emptyset
+    else Regex.emptyset
 
-def evals {α: Type} {μ: Nat} [DecidableEq α] (g: Expr.Grammar μ α) (ifExprs: IfExprs μ α) (t: α): List (Expr μ α) :=
+def evals {α: Type} {μ: Nat} [DecidableEq α] (g: Grammar μ α Pred) (ifExprs: IfExprs μ α) (t: α): List (Rule μ α Pred) :=
   List.map (fun x => eval g x t) ifExprs
 
-theorem evals_nil_is_nil {α: Type} {μ: Nat} [DecidableEq α] (g: Expr.Grammar μ α) (a: α):
+theorem evals_nil_is_nil {α: Type} {μ: Nat} [DecidableEq α] (g: Grammar μ α Pred) (a: α):
   evals g (μ := μ) [] a = [] := by
   unfold evals
   simp
 
-theorem evals_concat_is_concat {α: Type} [DecidableEq α] (g: Expr.Grammar μ α) (xs ys: IfExprs μ α) (a: α):
+theorem evals_concat_is_concat {α: Type} [DecidableEq α] (g: Grammar μ α Pred) (xs ys: IfExprs μ α) (a: α):
   evals g (xs ++ ys) a = evals g xs a ++ evals g ys a := by
   unfold evals
   simp
