Validator/Learning/ImperativeBasic.lean
@@ -6,8 +6,9 @@ import Validator.Std.Except
 import Validator.Std.Hedge
 import Validator.Parser.TokenTree
 
-import Validator.Expr.Expr
+import Validator.Expr.Grammar
 import Validator.Expr.IfExpr
+import Validator.Expr.Regex
 
 import Validator.Derive.Enter
 import Validator.Learning.ImperativeLeave
@@ -15,7 +16,7 @@ import Validator.Learning.ImperativeLeave
 namespace ImperativeBasic
 
 -- foldLoop is a more readable version of List.foldlM for imperative programmers:
-private def foldLoop (deriv: Exprs μ α -> Hedge.Node α -> Except String (Exprs μ α)) (start: Exprs μ α) (hedge: Hedge α): Except String (Exprs μ α) := do
+private def foldLoop (deriv: Rules μ α Pred -> Hedge.Node α -> Except String (Rules μ α Pred)) (start: Rules μ α Pred) (hedge: Hedge α): Except String (Rules μ α Pred) := do
   let mut res := start
   for tree in hedge do
     match deriv res tree with
@@ -23,10 +24,10 @@ private def foldLoop (deriv: Exprs μ α -> Hedge.Node α -> Except String (Expr
     | Except.ok r => res := r
   return res
 
-def derive [DecidableEq α] (g: Expr.Grammar μ α) (xs: Exprs μ α) (tree: Hedge.Node α): Except String (Exprs μ α) :=
+def derive [DecidableEq α] (g: Grammar μ α Pred) (xs: Rules μ α Pred) (tree: Hedge.Node α): Except String (Rules μ α Pred) :=
   -- If all expressions are unescapable, then simply return without look at the input tree.
   -- An example of an unescapable expression is emptyset, since its derivative is always emptyset, no matter the input.
-  if List.all xs Expr.unescapable
+  if List.all xs Regex.unescapable
   then Except.ok xs
   else
     -- Desconstruct the tree to retrieve its label and children
@@ -35,21 +36,21 @@ def derive [DecidableEq α] (g: Expr.Grammar μ α) (xs: Exprs μ α) (tree: Hed
       -- enters is one of our two new memoizable functions.
       let ifexprs: IfExprs μ α := Enter.deriveEnter xs
       -- childxs = expressions to evaluate on children.
-      let childxs: Exprs μ α := IfExpr.evals g ifexprs label
+      let childxs: Rules μ α Pred := IfExpr.evals g ifexprs label
       -- dchildxs = derivatives of children. The ' is for the exception it is wrapped in.
       -- see foldLoop for an explanation of what List.foldM does.
-      let dchildxs': Except String (Exprs μ α) := List.foldlM (derive g) childxs children
+      let dchildxs': Except String (Rules μ α Pred) := List.foldlM (derive g) childxs children
       match dchildxs' with
       | Except.error err => Except.error err
       | Except.ok dchildxs =>
       -- dxs = derivatives of xs. The ' is for the exception it is wrapped in.
       -- leaves is the other one of our two new memoizable functions.
-      let dxs': Except String (Exprs μ α) := ImperativeLeave.deriveLeave xs (List.map Expr.nullable dchildxs)
+      let dxs': Except String (Rules μ α Pred) := ImperativeLeave.deriveLeave xs (List.map Regex.nullable dchildxs)
       match dxs' with
       | Except.error err => Except.error err
       | Except.ok dxs => Except.ok dxs
 
-def derivs [DecidableEq α] (g: Expr.Grammar μ α) (x: Expr μ α) (hedge: Hedge α): Except String (Expr μ α) :=
+def derivs [DecidableEq α] (g: Grammar μ α Pred) (x: Rule μ α Pred) (hedge: Hedge α): Except String (Rule μ α Pred) :=
   -- see foldLoop for an explanation of what List.foldM does.
   let dxs := List.foldlM (derive g) [x] hedge
   match dxs with
@@ -57,75 +58,74 @@ def derivs [DecidableEq α] (g: Expr.Grammar μ α) (x: Expr μ α) (hedge: Hedg
   | Except.ok [dx] => Except.ok dx
   | Except.ok _ => Except.error "expected one expression"
 
-def validate [DecidableEq α] (g: Expr.Grammar μ α) (x: Expr μ α) (hedge: Hedge α): Except String Bool :=
+def validate [DecidableEq α] (g: Grammar μ α Pred) (x: Rule μ α Pred) (hedge: Hedge α): Except String Bool :=
   match derivs g x hedge with
   | Except.error err => Except.error err
-  | Except.ok x' => Except.ok (Expr.nullable x')
+  | Except.ok x' => Except.ok (Rule.nullable x')
 
-def run [DecidableEq α] (g: Expr.Grammar μ α) (t: Hedge.Node α): Except String Bool :=
-  validate g g.lookup0 [t]
+def run [DecidableEq α] (g: Grammar μ α Pred) (t: Hedge.Node α): Except String Bool :=
+  validate g g.start [t]
 
 -- Tests
--- Lean can use #guard to run these tests at compile time.
 
 open TokenTree (node)
 
 #guard run
-  (Expr.Grammar.singleton Expr.emptyset)
+  (Grammar.singleton Regex.emptyset)
   (node "a" [node "b" [], node "c" [node "d" []]]) =
   Except.ok false
 
 #guard run
-  (Expr.Grammar.mk (μ := 2)
-    (Expr.tree (Pred.eq (Token.string "a")) 1)
-    #v[Expr.epsilon]
+  (Grammar.mk (μ := 1)
+    (Regex.symbol (Pred.eq (Token.string "a"), 0))
+    #v[Regex.emptystr]
   )
   (node "a" []) =
   Except.ok true
 
 #guard run
-  (Expr.Grammar.mk (μ := 2)
-    (Expr.tree (Pred.eq (Token.string "a")) 1)
-    #v[Expr.epsilon]
+  (Grammar.mk (μ := 1)
+    (Regex.symbol (Pred.eq (Token.string "a"), 0))
+    #v[Regex.emptystr]
   )
   (node "a" [node "b" []]) =
   Except.ok false
 
 #guard run
-  (Expr.Grammar.mk (μ := 3)
-    (Expr.tree (Pred.eq (Token.string "a")) 1)
+  (Grammar.mk (μ := 2)
+    (Regex.symbol (Pred.eq (Token.string "a"), 0))
     #v[
-      (Expr.tree (Pred.eq (Token.string "b")) 2)
-      , Expr.epsilon
+      (Regex.symbol (Pred.eq (Token.string "b"), 1))
+      , Regex.emptystr
     ]
   )
   (node "a" [node "b" []])
   = Except.ok true
 
 #guard run
-  (Expr.Grammar.mk (μ := 3)
-    (Expr.tree (Pred.eq (Token.string "a")) 1)
+  (Grammar.mk (μ := 2)
+    (Regex.symbol (Pred.eq (Token.string "a"), 0))
     #v[
-      (Expr.concat
-        (Expr.tree (Pred.eq (Token.string "b")) 2)
-        (Expr.tree (Pred.eq (Token.string "c")) 2)
+      (Regex.concat
+        (Regex.symbol (Pred.eq (Token.string "b"), 1))
+        (Regex.symbol (Pred.eq (Token.string "c"), 1))
       )
-      , Expr.epsilon
+      , Regex.emptystr
     ]
   )
   (node "a" [node "b" [], node "c" []]) =
   Except.ok true
 
 #guard run
-  (Expr.Grammar.mk (μ := 4)
-    (Expr.tree (Pred.eq (Token.string "a")) 1)
+  (Grammar.mk (μ := 3)
+    (Regex.symbol (Pred.eq (Token.string "a"), 0))
     #v[
-      (Expr.concat
-        (Expr.tree (Pred.eq (Token.string "b")) 2)
-        (Expr.tree (Pred.eq (Token.string "c")) 3)
+      (Regex.concat
+        (Regex.symbol (Pred.eq (Token.string "b"), 1))
+        (Regex.symbol (Pred.eq (Token.string "c"), 2))
       )
-      , Expr.epsilon
-      , (Expr.tree (Pred.eq (Token.string "d")) 2)
+      , Regex.emptystr
+      , (Regex.symbol (Pred.eq (Token.string "d"), 1))
     ]
   )
   (node "a" [node "b" [], node "c" [node "d" []]]) =
