Validator/Validator/Validate.lean
@@ -4,8 +4,9 @@
 -- It does add compression for a small optimization, see lines marked with NEW
 
 import Validator.Expr.Compress
-import Validator.Expr.Expr
+import Validator.Expr.Grammar
 import Validator.Expr.IfExpr
+import Validator.Expr.Regex
 
 import Validator.Derive.Enter
 import Validator.Derive.Leave
@@ -20,19 +21,19 @@ import Validator.Validator.Inst.TreeParserMemM
 
 namespace Validate
 
-def deriveEnter [DecidableEq α] [ValidateM m μ α] (g: Expr.Grammar μ α) (xs: Exprs μ α): m (Exprs μ α) := do
+def deriveEnter [DecidableEq α] [ValidateM m μ α] (g: Grammar μ α Pred) (xs: Rules μ α Pred): m (Rules μ α Pred) := do
   let token <- Parser.token
   let enters <- Enter.DeriveEnter.deriveEnter xs
   return IfExpr.evals g enters token
 
-def deriveLeaveM [ValidateM m μ α] (xs: Exprs μ α) (cs: Exprs μ α): m (Exprs μ α) :=
-  Leave.DeriveLeaveM.deriveLeaveM xs (List.map Expr.nullable cs)
+def deriveLeaveM [ValidateM m μ α] (xs: Rules μ α Pred) (cs: Rules μ α Pred): m (Rules μ α Pred) :=
+  Leave.DeriveLeaveM.deriveLeaveM xs (List.map Rule.nullable cs)
 
-def deriveValue [DecidableEq α] [ValidateM m μ α] (g: Expr.Grammar μ α) (xs: Exprs μ α): m (Exprs μ α) := do
+def deriveValue [DecidableEq α] [ValidateM m μ α] (g: Grammar μ α Pred) (xs: Rules μ α Pred): m (Rules μ α Pred) := do
   deriveLeaveM xs (<- deriveEnter g xs)
 
-partial def derive [DecidableEq α] [ValidateM m μ α] (g: Expr.Grammar μ α) (xs: Exprs μ α): m (Exprs μ α) := do
-  if List.all xs Expr.unescapable then
+partial def derive [DecidableEq α] [ValidateM m μ α] (g: Grammar μ α Pred) (xs: Rules μ α Pred): m (Rules μ α Pred) := do
+  if List.all xs Regex.unescapable then
     Parser.skip; return xs
   match <- Parser.next with
   | Hint.field =>
@@ -56,75 +57,75 @@ partial def derive [DecidableEq α] [ValidateM m μ α] (g: Expr.Grammar μ α) 
   | Hint.leave => return xs -- never happens at the top
   | Hint.eof => return xs -- only happens at the top
 
-def validate {m} {μ: Nat} {α: Type} [DecidableEq α] [ValidateM m μ α] (g: Expr.Grammar μ α) (x: Expr μ α): m Bool := do
+def validate {m} {μ: Nat} {α: Type} [DecidableEq α] [ValidateM m μ α] (g: Grammar μ α Pred) (x: Rule μ α Pred): m Bool := do
   let dxs <- derive g [x]
   match dxs with
-  | [dx] => return Expr.nullable dx
+  | [dx] => return Rule.nullable dx
   | _ => throw "expected one expression"
 
-def run {μ: Nat} {α: Type} [DecidableEq α] [Hashable α] (g: Expr.Grammar μ α) (t: Hedge.Node α): Except String Bool :=
-  TreeParserMemM.run' (μ := μ) (validate g g.lookup0) t
+def run {μ: Nat} {α: Type} [DecidableEq α] [Hashable α] (g: Grammar μ α Pred) (t: Hedge.Node α): Except String Bool :=
+  TreeParserMemM.run' (μ := μ) (validate g g.start) t
 
 -- Tests
 
 open TokenTree (node)
 
 #guard run
-  (Expr.Grammar.singleton Expr.emptyset)
+  (Grammar.singleton Regex.emptyset)
   (node "a" [node "b" [], node "c" [node "d" []]]) =
   Except.ok false
 
 #guard run
-  (Expr.Grammar.mk (μ := 2)
-    (Expr.tree (Pred.eq (Token.string "a")) 1)
-    #v[Expr.epsilon]
+  (Grammar.mk (μ := 1)
+    (Regex.symbol (Pred.eq (Token.string "a"), 0))
+    #v[Regex.emptystr]
   )
   (node "a" []) =
   Except.ok true
 
 #guard run
-  (Expr.Grammar.mk (μ := 2)
-    (Expr.tree (Pred.eq (Token.string "a")) 1)
-    #v[Expr.epsilon]
+  (Grammar.mk (μ := 1)
+    (Regex.symbol (Pred.eq (Token.string "a"), 0))
+    #v[Regex.emptystr]
   )
   (node "a" [node "b" []]) =
   Except.ok false
 
 #guard run
-  (Expr.Grammar.mk (μ := 3)
-    (Expr.tree (Pred.eq (Token.string "a")) 1)
+  (Grammar.mk (μ := 2)
+    (Regex.symbol (Pred.eq (Token.string "a"), 0))
     #v[
-      (Expr.tree (Pred.eq (Token.string "b")) 2)
-      , Expr.epsilon
+      (Regex.symbol (Pred.eq (Token.string "b"), 1))
+      , Regex.emptystr
     ]
   )
   (node "a" [node "b" []])
   = Except.ok true
 
 #guard run
-  (Expr.Grammar.mk (μ := 3)
-    (Expr.tree (Pred.eq (Token.string "a")) 1)
+  (Grammar.mk (μ := 2)
+    (Regex.symbol (Pred.eq (Token.string "a"), 0))
     #v[
-      (Expr.concat
-        (Expr.tree (Pred.eq (Token.string "b")) 2)
-        (Expr.tree (Pred.eq (Token.string "c")) 2)
+      (Regex.concat
+        (Regex.symbol (Pred.eq (Token.string "b"), 1))
+        (Regex.symbol (Pred.eq (Token.string "c"), 1))
       )
-      , Expr.epsilon
+      , Regex.emptystr
     ]
   )
   (node "a" [node "b" [], node "c" []]) =
   Except.ok true
 
 #guard run
-  (Expr.Grammar.mk (μ := 4)
-    (Expr.tree (Pred.eq (Token.string "a")) 1)
+  (Grammar.mk (μ := 3)
+    (Regex.symbol (Pred.eq (Token.string "a"), 0))
     #v[
-      (Expr.concat
-        (Expr.tree (Pred.eq (Token.string "b")) 2)
-        (Expr.tree (Pred.eq (Token.string "c")) 3)
+      (Regex.concat
+        (Regex.symbol (Pred.eq (Token.string "b"), 1))
+        (Regex.symbol (Pred.eq (Token.string "c"), 2))
       )
-      , Expr.epsilon
-      , (Expr.tree (Pred.eq (Token.string "d")) 2)
+      , Regex.emptystr
+      , (Regex.symbol (Pred.eq (Token.string "d"), 1))
     ]
   )
   (node "a" [node "b" [], node "c" [node "d" []]]) =
@@ -132,81 +133,69 @@ open TokenTree (node)
 
 -- try to engage skip using emptyset, since it is unescapable
 #guard run
-  (Expr.Grammar.mk (μ := 2)
-    (Expr.tree (Pred.eq (Token.string "a")) 1)
-    #v[Expr.emptyset]
+  (Grammar.mk (μ := 1)
+    (Regex.symbol (Pred.eq (Token.string "a"), 0))
+    #v[Regex.emptyset]
   )
   (node "a" [node "b" []])
   = Except.ok false
 
 #guard run
-  (Expr.Grammar.mk (μ := 5)
-    (Expr.tree (Pred.eq (Token.string "a")) 1)
+  (Grammar.mk (μ := 4)
+    (Regex.symbol (Pred.eq (Token.string "a"), 0))
     #v[
-      (Expr.concat
-        (Expr.tree (Pred.eq (Token.string "b")) 4)
-        (Expr.tree (Pred.eq (Token.string "c")) 3)
+      (Regex.concat
+        (Regex.symbol (Pred.eq (Token.string "b"), 3))
+        (Regex.symbol (Pred.eq (Token.string "c"), 2))
       )
-      , Expr.epsilon
-      , (Expr.tree (Pred.eq (Token.string "d")) 2)
-      , Expr.emptyset
+      , Regex.emptystr
+      , (Regex.symbol (Pred.eq (Token.string "d"), 1))
+      , Regex.emptyset
     ]
   )
   (node "a" [node "b" [], node "c" [node "d" []]])
   = Except.ok false
 
 #guard run
-  (Expr.Grammar.mk (μ := 3)
-    (Expr.tree (Pred.eq (Token.string "a")) 1)
+  (Grammar.mk (μ := 2)
+    (Regex.symbol (Pred.eq (Token.string "a"), 0))
     #v[
-      (Expr.concat
-        (Expr.tree (Pred.eq (Token.string "b"))
-          2
-        )
-        Expr.emptyset
+      (Regex.concat
+        (Regex.symbol (Pred.eq (Token.string "b"), 1))
+        Regex.emptyset
       )
-      , Expr.epsilon
+      , Regex.emptystr
     ]
   )
   (node "a" [node "b" [], node "c" [node "d" []]]) =
   Except.ok false
 
 #guard run
-  (Expr.Grammar.mk (μ := 4)
-    (Expr.tree (Pred.eq (Token.string "a")) 1)
+  (Grammar.mk (μ := 3)
+    (Regex.symbol (Pred.eq (Token.string "a"), 0))
     #v[
-      (Expr.concat
-        (Expr.tree (Pred.eq (Token.string "b"))
-          2
-        )
-        (Expr.tree (Pred.eq (Token.string "c"))
-          3
-        )
+      (Regex.concat
+        (Regex.symbol (Pred.eq (Token.string "b"), 1))
+        (Regex.symbol (Pred.eq (Token.string "c"), 2))
       )
-      , Expr.epsilon
-      , Expr.emptyset
+      , Regex.emptystr
+      , Regex.emptyset
     ]
   )
   (node "a" [node "b" [], node "c" [node "d" []]])
   = Except.ok false
 
 #guard run
-  (Expr.Grammar.mk (μ := 5)
-    (Expr.tree (Pred.eq (Token.string "a")) 1)
+  (Grammar.mk (μ := 4)
+    (Regex.symbol (Pred.eq (Token.string "a"), 0))
     #v[
-      (Expr.concat
-        (Expr.tree (Pred.eq (Token.string "b"))
-          1
-        )
-        (Expr.tree (Pred.eq (Token.string "c"))
-          2
-        )
+      (Regex.concat
+        (Regex.symbol (Pred.eq (Token.string "b"), 0))
+        (Regex.symbol (Pred.eq (Token.string "c"), 1))
       )
-      , Expr.epsilon
-      , (Expr.tree (Pred.eq (Token.string "d"))
-          3
-        )
-      , Expr.emptyset
+      , Regex.emptystr
+      , (Regex.symbol (Pred.eq (Token.string "d"), 2))
+      , Regex.emptyset
     ]
   )
   (node "a" [node "b" [], node "c" [node "d" []]])
