Validator/Learning/ImperativeLeave.lean
@@ -1,31 +1,32 @@
 -- ImperativeLeave.lean is an implementation of Leave.lean that does not use monads, so it is more verbose.
 -- This is supposed to make it easier to understand for programmers that have not used monads before.
 
-import Validator.Expr.Expr
+import Validator.Expr.Grammar
+import Validator.Expr.Regex
 
 namespace ImperativeLeave
 
-def leave (x: Expr μ α) (ns: List Bool): Except String (Expr μ α × List Bool) :=
+def leave (x: Rule μ α Pred) (ns: List Bool): Except String (Rule μ α Pred × List Bool) :=
   match x with
-  | Expr.emptyset => Except.ok (Expr.emptyset, ns)
-  | Expr.epsilon => Except.ok (Expr.emptyset, ns)
-  | Expr.tree _ _ =>
+  | Regex.emptyset => Except.ok (Regex.emptyset, ns)
+  | Regex.emptystr => Except.ok (Regex.emptyset, ns)
+  | Regex.symbol _ =>
     match ns with
     | [] => Except.error "wtf"
     | (null::ns') =>
       if null
-      then Except.ok (Expr.epsilon, ns')
-      else Except.ok (Expr.emptyset, ns')
-  | Expr.or y z =>
+      then Except.ok (Regex.emptystr, ns')
+      else Except.ok (Regex.emptyset, ns')
+  | Regex.or y z =>
     match leave y ns with
     | Except.error e => Except.error e
     | Except.ok (y', ns') =>
       match leave z ns' with
       | Except.error e => Except.error e
       | Except.ok (z', ns'') =>
-        Except.ok (Expr.or y' z', ns'')
-  | Expr.concat y z =>
-    if Expr.nullable y
+        Except.ok (Regex.or y' z', ns'')
+  | Regex.concat y z =>
+    if Regex.nullable y
     then
       match leave y ns with
       | Except.error e => Except.error e
@@ -33,34 +34,34 @@ def leave (x: Expr μ α) (ns: List Bool): Except String (Expr μ α × List Boo
         match leave z ns' with
         | Except.error e => Except.error e
         | Except.ok (z', ns'') =>
-          Except.ok (Expr.or (Expr.concat y' z) z', ns'')
+          Except.ok (Regex.or (Regex.concat y' z) z', ns'')
     else
       match leave y ns with
       | Except.error e => Except.error e
       | Except.ok (y', ns') =>
-        Except.ok (Expr.concat y' z, ns')
-  | Expr.star y =>
+        Except.ok (Regex.concat y' z, ns')
+  | Regex.star y =>
       match leave y ns with
       | Except.error e => Except.error e
       | Except.ok (y', ns') =>
-        Except.ok (Expr.star y', ns')
+        Except.ok (Regex.star y', ns')
 
 -- deriveLeave takes a list of expressions and list of bools.
 -- The list of bools represent the nullability of the derived child expressions.
 -- Each bool will then replace each tree expression with either an epsilon or emptyset.
 -- The lists do not to be the same length, because each expression can contain an arbitrary number of tree expressions.
-def deriveLeave (xs: Exprs μ α) (ns: List Bool): Except String (Exprs μ α) :=
+def deriveLeave (xs: Rules μ α Pred) (ns: List Bool): Except String (Rules μ α Pred) :=
   match xs with
   | [] =>
     match ns with
     | [] => Except.ok []
     | _ => Except.error "Not all nulls were consumed, but there are no expressions to place them in."
   | (x::xs') =>
-    let lx': Except String (Expr μ α × List Bool) := leave x ns
+    let lx': Except String (Rule μ α Pred × List Bool) := leave x ns
     match lx' with
     | Except.error err => Except.error err
     | Except.ok (lx, tailns) =>
-    let lxs': Except String (Exprs μ α) := deriveLeave xs' tailns
+    let lxs': Except String (Rules μ α Pred) := deriveLeave xs' tailns
     match lxs' with
     | Except.error err => Except.error err
     | Except.ok lxs =>
