Validator/Memoize/MemLeave.lean
@@ -2,12 +2,13 @@ import Std
 
 import Validator.Std.Debug
 
-import Validator.Expr.Expr
+import Validator.Expr.Grammar
 import Validator.Expr.IfExpr
+import Validator.Expr.Regex
 
 import Validator.Derive.Leave
 
-abbrev MemLeave.LeaveMap μ α [DecidableEq α] [Hashable α] := Std.ExtHashMap (Exprs μ α × List Bool) (Exprs μ α)
+abbrev MemLeave.LeaveMap μ α [DecidableEq α] [Hashable α] := Std.ExtHashMap (Rules μ α Pred × List Bool) (Rules μ α Pred)
 def MemLeave.LeaveMap.mk [DecidableEq α] [Hashable α]: LeaveMap μ α := Std.ExtHashMap.emptyWithCapacity
 
 class MemLeave (m: Type -> Type u) (μ: outParam Nat) (α: outParam Type) [DecidableEq α] [Hashable α] where
@@ -19,7 +20,7 @@ namespace MemLeave
 def deriveLeaveM
   [DecidableEq α] [Hashable α]
   [Monad m] [Debug m] [MonadExcept String m] [MemLeave m μ α]
-  (xs: Exprs μ α) (ns: List Bool): m (Exprs μ α) := do
+  (xs: Rules μ α Pred) (ns: List Bool): m (Rules μ α Pred) := do
   let memoized <- MemLeave.getLeave
   match memoized.get? (xs, ns) with
   | Option.none =>
@@ -32,4 +33,4 @@ def deriveLeaveM
     return value
 
 instance [DecidableEq α] [Hashable α] [Monad m] [Debug m] [MonadExcept String m] [MemLeave m μ α] : Leave.DeriveLeaveM m μ α where
-  deriveLeaveM (xs: Exprs μ α) (ns: List Bool): m (Exprs μ α) := deriveLeaveM xs ns
+  deriveLeaveM (xs: Rules μ α Pred) (ns: List Bool): m (Rules μ α Pred) := deriveLeaveM xs ns
